\parte{}
\[
    E(X_{(n)}) = \int_{-\infty}^{\infty}
    {\alpha_n x f(x)F(x)^{n-1}(1-F(x))^{N-n}}dx
\]
که $\alpha_n = \frac{n!}{(N-n)!(n-1)!}$
.\\\\
\parte{}
\[
    E(X_{(n)}) = \int_{-\infty}^{\infty}
    {\alpha_n x f(x)F(x)^{n-1}(1-F(x))^{N-n}}dx
\]
\[
    = \int_{-\infty}^{\infty}
    {\alpha_n (u+\alpha) f((u+\alpha))F((u+\alpha))^{n-1}(1-F((u+\alpha)))^{N-n}}du
\]
\[
    = \int_{-\infty}^{\infty}
    {\alpha_n (u+\alpha) g(u)G(u)^{n-1}(1-G(u))^{N-n}}du
\]

\parte{}

\[
    E(X_{(n)}) = \int_{-\infty}^{\infty}
    {\alpha_n (u+\alpha) g(u)G(u)^{n-1}(1-G(u))^{N-n}}du
\]
\[
    = \alpha_n  \int_{-\infty}^{\infty}
    {u g(u)G(u)^{n-1}(1-G(u))^{N-n}}du
    +
    \int_{-\infty}^{\infty}
    {\alpha_n \alpha g(u)G(u)^{n-1}(1-G(u))^{N-n}}du
\]\\

که تابع $g(u)G(u)^{n-1}(1-G(u))^{N-n}$
زوج است.(زیرا تمام توابع آن زوج اند).\\\\
پس تابع $ug(u)G(u)^{n-1}(1-G(u))^{N-n}$
یک تابع فرد است .\\\\
در نتیجه 
$\int_{-\infty}^{\infty}
{u g(u)G(u)^{n-1}(1-G(u))^{N-n}}du = 0$
پس داریم:\\

\[
    E(X_{(n)}) = \int_{-\infty}^{\infty}
    {\alpha_n \alpha g(u)G(u)^{n-1}(1-G(u))^{N-n}}du
\]
\[
    = \alpha \int_{-\infty}^{\infty}
    {\alpha_ng(u)G(u)^{n-1}(1-G(u))^{N-n}}du
\]\\
که عبارت $\int_{-\infty}^{\infty}
{\alpha_ng(u)G(u)^{n-1}(1-G(u))^{N-n}}du$
همان تابع چگالی توزیع میانه است و درنتیجه این انتگرال برابر 
$1$ است پس :\\
\[
    E(X_{(n)}) = \alpha \int_{-\infty}^{\infty}
    {\alpha_ng(u)G(u)^{n-1}(1-G(u))^{N-n}}du = 
    \alpha
\]\\