\parte{}
تغییر متغیر $u = G(x)$ را انجام میدهیم داریم:\\
\[
    u = G(x)
    \quad
    =>
    \quad
    \frac{du}{dx} = g(x)
    \quad
    =>
    \quad
    dx = \frac{du}{g(x)}
\]
حالا عبارات بدست آمده را در انتگرال جایگذاری میکنیم داریم:\\
\[
    var(X_{(n)}) = \int_{-\infty}^{\infty}{
    \alpha_n {H(u)}^2(u(1-u))^{n-1} du
  }
\]

\parte{}
\[
    H(u) = H(\frac{1}{2})+{H^{\prime}(\frac{1}{2})}(u-\frac{1}{2}) 
\]
\parte{}
 قرار می دهیم $H(\frac{1}{2}) = a$و $H(\frac{1}{2}) = b$.

\[
    var(X_{(n)}) = \alpha_n  \int_{-\infty}^{\infty}{
    {(a+b(u-\frac{1}{2}))}^2(u(1-u))^{n-1} du
  }
\]
\[
    = \alpha_n  \int_{-\infty}^{\infty}{
    {(a+b(\frac{z}{2}))}^2(\frac{z+1}{2}(1-\frac{z+1}{2}))^{n-1} \frac{dz}{2}
  }
\]

\[
    = \alpha_n  \int_{-\infty}^{\infty}{
    (a^2+\frac{b^2z^2}{4}+abz)
    (\frac{z+1}{2} - \frac{z^2+2z+1}{4})^{n-1}
     \frac{dz}{2}
  }
\]
\[
    = \alpha_n  \int_{-\infty}^{\infty}{
    (a^2+\frac{b^2y}{4}+aby^\frac{1}{2})
    (\frac{y^\frac{1}{2}+1}{2} - \frac{y+2y^\frac{1}{2}+1}{4})^{n-1}
     \frac{dy}{4z}
  }
\]

% \[
%     = \alpha_n  \int_{-\infty}^{\infty}{
%     (a^2 + b^2(u^2 + \frac{1}{4} - u)+2ab(u-\frac{1}{2}))
%     (u(1-u))^{n-1} du
%   }
% \]